keep the last version of allInstances
git-svn-id: https://projects.brucker.ch/hol-testgen/svn/HOL-TestGen/trunk/hol-testgen@9814 3260e6d1-4efc-4170-b0a7-36055960796d

examples/Employee_DesignModel_UMLPart.thy
@@ -117,27 +117,19 @@ definition OclAny :: "\<AA> \<Rightarrow> oclany"
 where     "OclAny \<equiv> (the_inv in\<^isub>o\<^isub>c\<^isub>l\<^isub>a\<^isub>n\<^isub>y)"
 *)
 
-fun    Person :: "\<AA> \<Rightarrow> person"
-where "Person (in\<^isub>o\<^isub>c\<^isub>l\<^isub>a\<^isub>n\<^isub>y(mk\<^isub>o\<^isub>c\<^isub>l\<^isub>a\<^isub>n\<^isub>y oid \<lfloor>(a,b)\<rfloor>)) = mk\<^isub>p\<^isub>e\<^isub>r\<^isub>s\<^isub>o\<^isub>n oid a b"
-    | "Person (in\<^isub>p\<^isub>e\<^isub>r\<^isub>s\<^isub>o\<^isub>n(mk\<^isub>p\<^isub>e\<^isub>r\<^isub>s\<^isub>o\<^isub>n oid a b)) = mk\<^isub>p\<^isub>e\<^isub>r\<^isub>s\<^isub>o\<^isub>n oid a b"
-
-fun    OclAny :: "\<AA> \<Rightarrow> oclany"
-where "OclAny (in\<^isub>o\<^isub>c\<^isub>l\<^isub>a\<^isub>n\<^isub>y X) = X"
-     |"OclAny (in\<^isub>p\<^isub>e\<^isub>r\<^isub>s\<^isub>o\<^isub>n (mk\<^isub>p\<^isub>e\<^isub>r\<^isub>s\<^isub>o\<^isub>n oid a b)) = mk\<^isub>o\<^isub>c\<^isub>l\<^isub>a\<^isub>n\<^isub>y oid \<lfloor>(a,b)\<rfloor>"
-
-definition    Person' :: "\<AA> \<Rightarrow> person option"
-where "Person' = (\<lambda>x. case x of
+definition    Person :: "\<AA> \<Rightarrow> person option"
+where "Person = (\<lambda>x. case x of
       in\<^isub>o\<^isub>c\<^isub>l\<^isub>a\<^isub>n\<^isub>y (mk\<^isub>o\<^isub>c\<^isub>l\<^isub>a\<^isub>n\<^isub>y oid \<lfloor>(a,b)\<rfloor>) \<Rightarrow> \<lfloor>mk\<^isub>p\<^isub>e\<^isub>r\<^isub>s\<^isub>o\<^isub>n oid a b\<rfloor>
     | in\<^isub>p\<^isub>e\<^isub>r\<^isub>s\<^isub>o\<^isub>n (mk\<^isub>p\<^isub>e\<^isub>r\<^isub>s\<^isub>o\<^isub>n oid a b) \<Rightarrow> \<lfloor>mk\<^isub>p\<^isub>e\<^isub>r\<^isub>s\<^isub>o\<^isub>n oid a b\<rfloor>
     | _ \<Rightarrow> None)"
 
-definition    OclAny' :: "\<AA> \<Rightarrow> oclany option"
-where "OclAny' = (\<lambda>x. case x of
+definition    OclAny :: "\<AA> \<Rightarrow> oclany option"
+where "OclAny = (\<lambda>x. case x of
       in\<^isub>o\<^isub>c\<^isub>l\<^isub>a\<^isub>n\<^isub>y X \<Rightarrow> \<lfloor>X\<rfloor>
     | in\<^isub>p\<^isub>e\<^isub>r\<^isub>s\<^isub>o\<^isub>n (mk\<^isub>p\<^isub>e\<^isub>r\<^isub>s\<^isub>o\<^isub>n oid a b) \<Rightarrow> \<lfloor>mk\<^isub>o\<^isub>c\<^isub>l\<^isub>a\<^isub>n\<^isub>y oid \<lfloor>(a,b)\<rfloor>\<rfloor>)"
 
-lemma oclany_none: "OclAny' x \<noteq> None"
- apply(simp add: OclAny'_def)
+lemma OclAny_some: "OclAny x \<noteq> None"
+ apply(simp add: OclAny_def)
  apply(case_tac x, simp_all)
  apply(case_tac person, simp_all)
 done
@@ -221,25 +213,17 @@ section{* OclAllInstances *}
 (* IS THIS WHAT WE WANT ? THIS DEFINITION FILTERS OBJECTS THAT ARE BOOKED UNDER
 THEIR APPARENT (STATIC) TYPE INTO THE CONTEXT, NOT BY THEIR ACTUAL (DYNAMIC) TYPE. *)
 lemma "Person .allInstances() =
-             (\<lambda>\<tau>.  Abs_Set_0 \<lfloor>\<lfloor>(Some \<circ> Some \<circ> Person_sumC)`(ran(heap(snd \<tau>))) \<rfloor>\<rfloor>) "
-by(rule ext, simp add:OclAllInstances_def Person_def)
-
-lemma "OclAllInstances' Person' =
-             (\<lambda>\<tau>.  Abs_Set_0  \<lfloor>\<lfloor>Some ` (Person' ` ran (heap (snd \<tau>)) - {None})\<rfloor>\<rfloor>) "
-by(rule ext, simp add:OclAllInstances'_def)
+             (\<lambda>\<tau>.  Abs_Set_0  \<lfloor>\<lfloor>Some ` (Person ` ran (heap (snd \<tau>)) - {None})\<rfloor>\<rfloor>) "
+by(rule ext, simp add:OclAllInstances_at_post_def)
 
 lemma "Person .allInstances@pre() = 
-             (\<lambda>\<tau>.  Abs_Set_0 \<lfloor>\<lfloor>(Some \<circ> Some \<circ> Person_sumC)`(ran(heap(fst \<tau>))) \<rfloor>\<rfloor>) "
-by(rule ext, simp add:OclAllInstances_at_pre_def Person_def)
+             (\<lambda>\<tau>.  Abs_Set_0  \<lfloor>\<lfloor>Some ` (Person ` ran (heap (fst \<tau>)) - {None})\<rfloor>\<rfloor>) "
+by(rule ext, simp add:OclAllInstances_at_pre_def)
 
 lemma "OclAny .allInstances() =
-             (\<lambda>\<tau>.  Abs_Set_0 \<lfloor>\<lfloor>(Some \<circ> Some \<circ> OclAny_sumC)`(ran(heap(snd \<tau>))) \<rfloor>\<rfloor>) "
-by(rule ext, simp add:OclAllInstances_def OclAny_def)
-
-lemma "OclAllInstances' OclAny' =
-             (\<lambda>\<tau>.  Abs_Set_0  \<lfloor>\<lfloor> Some ` OclAny' ` ran (heap (snd \<tau>)) \<rfloor>\<rfloor>) "
- apply(rule ext, simp add: OclAllInstances'_def)
- apply(subgoal_tac " (OclAny' ` ran (heap (snd \<tau>)) - {None}) = (OclAny' ` ran (heap (snd \<tau>)))", simp)
+             (\<lambda>\<tau>.  Abs_Set_0  \<lfloor>\<lfloor> Some ` OclAny ` ran (heap (snd \<tau>)) \<rfloor>\<rfloor>) "
+ apply(rule ext, simp add: OclAllInstances_at_post_def)
+ apply(subgoal_tac " (OclAny ` ran (heap (snd \<tau>)) - {None}) = (OclAny ` ran (heap (snd \<tau>)))", simp)
  apply(simp add: image_def)
  apply(rule equalityI)
  apply(rule subsetI)
@@ -247,13 +231,24 @@ lemma "OclAllInstances' OclAny' =
  apply(rule subsetI)
  apply(simp)
  apply(drule bexE) prefer 2 apply assumption
- apply(case_tac x, metis oclany_none)
+ apply(case_tac x, metis OclAny_some)
  apply(blast)
 done
 
-lemma "OclAny .allInstances@pre() = 
-             (\<lambda>\<tau>.  Abs_Set_0 \<lfloor>\<lfloor>(Some \<circ> Some \<circ> OclAny_sumC)`(ran(heap(fst \<tau>))) \<rfloor>\<rfloor>) "
-by(rule ext, simp add:OclAllInstances_at_pre_def OclAny_def)
+lemma "OclAny .allInstances@pre() =
+             (\<lambda>\<tau>.  Abs_Set_0  \<lfloor>\<lfloor> Some ` OclAny ` ran (heap (fst \<tau>)) \<rfloor>\<rfloor>) "
+ apply(rule ext, simp add: OclAllInstances_at_pre_def)
+ apply(subgoal_tac " (OclAny ` ran (heap (fst \<tau>)) - {None}) = (OclAny ` ran (heap (fst \<tau>)))", simp)
+ apply(simp add: image_def)
+ apply(rule equalityI)
+ apply(rule subsetI)
+ apply (metis (lifting) Diff_iff)
+ apply(rule subsetI)
+ apply(simp)
+ apply(drule bexE) prefer 2 apply assumption
+ apply(case_tac x, metis OclAny_some)
+ apply(blast)
+done
 
 
 text{* For each Class \emph{C}, we will have a casting operation \verb+.oclAsType(+\emph{C}\verb+)+,
@@ -271,6 +266,9 @@ subsection{* Definition *}
 consts OclAsType\<^isub>o\<^isub>c\<^isub>l\<^isub>a\<^isub>n\<^isub>y :: "'\<alpha> \<Rightarrow> OclAny" ("(_) .oclAsType'(OclAny')")
 consts OclAsType\<^isub>p\<^isub>e\<^isub>r\<^isub>s\<^isub>o\<^isub>n :: "'\<alpha> \<Rightarrow> Person" ("(_) .oclAsType'(Person')")
 
+definition "OclAsType\<^isub>o\<^isub>c\<^isub>l\<^isub>a\<^isub>n\<^isub>y_\<AA> u = \<lfloor>case u of in\<^isub>o\<^isub>c\<^isub>l\<^isub>a\<^isub>n\<^isub>y a \<Rightarrow> a 
+                                          | in\<^isub>p\<^isub>e\<^isub>r\<^isub>s\<^isub>o\<^isub>n (mk\<^isub>p\<^isub>e\<^isub>r\<^isub>s\<^isub>o\<^isub>n oid a b) \<Rightarrow> mk\<^isub>o\<^isub>c\<^isub>l\<^isub>a\<^isub>n\<^isub>y oid \<lfloor>(a,b)\<rfloor>\<rfloor>"
+
 defs (overloaded) OclAsType\<^isub>o\<^isub>c\<^isub>l\<^isub>a\<^isub>n\<^isub>y_OclAny: 
         "(X::OclAny) .oclAsType(OclAny) \<equiv> X" 
 
@@ -280,6 +278,10 @@ defs (overloaded) OclAsType\<^isub>o\<^isub>c\<^isub>l\<^isub>a\<^isub>n\<^isub>
                               \<bottom>   \<Rightarrow> invalid \<tau>
                             | \<lfloor>\<bottom>\<rfloor> \<Rightarrow> null \<tau>    
                             | \<lfloor>\<lfloor>mk\<^isub>p\<^isub>e\<^isub>r\<^isub>s\<^isub>o\<^isub>n oid a b \<rfloor>\<rfloor> \<Rightarrow>  \<lfloor>\<lfloor>  (mk\<^isub>o\<^isub>c\<^isub>l\<^isub>a\<^isub>n\<^isub>y oid \<lfloor>(a,b)\<rfloor>) \<rfloor>\<rfloor>)"
+
+definition "OclAsType\<^isub>p\<^isub>e\<^isub>r\<^isub>s\<^isub>o\<^isub>n_\<AA> u = (case u of in\<^isub>p\<^isub>e\<^isub>r\<^isub>s\<^isub>o\<^isub>n p \<Rightarrow> \<lfloor>p\<rfloor> 
+                                          | in\<^isub>o\<^isub>c\<^isub>l\<^isub>a\<^isub>n\<^isub>y (mk\<^isub>o\<^isub>c\<^isub>l\<^isub>a\<^isub>n\<^isub>y oid \<lfloor>(a,b)\<rfloor>) \<Rightarrow> \<lfloor>mk\<^isub>p\<^isub>e\<^isub>r\<^isub>s\<^isub>o\<^isub>n oid a b\<rfloor>
+                                          | _ \<Rightarrow> None)"
 
 defs (overloaded) OclAsType\<^isub>p\<^isub>e\<^isub>r\<^isub>s\<^isub>o\<^isub>n_OclAny: 
         "(X::OclAny) .oclAsType(Person) \<equiv> 
@@ -632,9 +634,6 @@ definition "eval_extract X f = (\<lambda> \<tau>. case X \<tau> of
                                | \<lfloor>\<lfloor> obj \<rfloor>\<rfloor> \<Rightarrow> f (oid_of obj) \<tau>)"
 
 (*
-definition "OclAsType\<^isub>p\<^isub>e\<^isub>r\<^isub>s\<^isub>o\<^isub>n_\<AA> u = (case u of in\<^isub>p\<^isub>e\<^isub>r\<^isub>s\<^isub>o\<^isub>n p \<Rightarrow>  p 
-                                          | in\<^isub>o\<^isub>c\<^isub>l\<^isub>a\<^isub>n\<^isub>y (mk\<^isub>o\<^isub>c\<^isub>l\<^isub>a\<^isub>n\<^isub>y oid \<lfloor>(a,b)\<rfloor>) \<Rightarrow> (mk\<^isub>p\<^isub>e\<^isub>r\<^isub>s\<^isub>o\<^isub>n oid a b))" *)
-(*
 definition "deref\<^isub>o\<^isub>i\<^isub>d fst_snd f oid = (\<lambda>\<tau>. case (heap (fst_snd \<tau>)) oid of
                        \<lfloor> in\<^isub>p\<^isub>e\<^isub>r\<^isub>s\<^isub>o\<^isub>n obj \<rfloor> \<Rightarrow> f obj \<tau>
                      | \<lfloor> in\<^isub>o\<^isub>c\<^isub>l\<^isub>a\<^isub>n\<^isub>y obj \<rfloor> \<Rightarrow> f obj \<tau>
@@ -983,7 +982,7 @@ value "\<And>\<sigma>\<^isub>1 \<sigma>\<^isub>1'.   (\<sigma>\<^isub>1,\<sigma>
 value "\<And>\<sigma>\<^isub>1 \<sigma>\<^isub>1'.   (\<sigma>\<^isub>1,\<sigma>\<^isub>1') \<Turnstile>      (X\<^isub>P\<^isub>e\<^isub>r\<^isub>s\<^isub>o\<^isub>n8 .oclIsKindOf(OclAny))"
 
 
-lemma "\<And>\<sigma>\<^isub>1.    (\<sigma>\<^isub>1,\<sigma>\<^isub>1') \<Turnstile>      (Person .allInstances() \<doteq> Set{ X\<^isub>P\<^isub>e\<^isub>r\<^isub>s\<^isub>o\<^isub>n1, X\<^isub>P\<^isub>e\<^isub>r\<^isub>s\<^isub>o\<^isub>n2, X\<^isub>P\<^isub>e\<^isub>r\<^isub>s\<^isub>o\<^isub>n3, X\<^isub>P\<^isub>e\<^isub>r\<^isub>s\<^isub>o\<^isub>n4(*, X\<^isub>P\<^isub>e\<^isub>r\<^isub>s\<^isub>o\<^isub>n5*), X\<^isub>P\<^isub>e\<^isub>r\<^isub>s\<^isub>o\<^isub>n6, X\<^isub>P\<^isub>e\<^isub>r\<^isub>s\<^isub>o\<^isub>n7 .oclAsType(Person), \<lambda>_. \<lfloor>\<lfloor>Person (in\<^isub>o\<^isub>c\<^isub>l\<^isub>a\<^isub>n\<^isub>y person8)\<rfloor>\<rfloor> })"
+lemma "\<And>\<sigma>\<^isub>1.    (\<sigma>\<^isub>1,\<sigma>\<^isub>1') \<Turnstile>      (Person .allInstances() \<doteq> Set{ X\<^isub>P\<^isub>e\<^isub>r\<^isub>s\<^isub>o\<^isub>n1, X\<^isub>P\<^isub>e\<^isub>r\<^isub>s\<^isub>o\<^isub>n2, X\<^isub>P\<^isub>e\<^isub>r\<^isub>s\<^isub>o\<^isub>n3, X\<^isub>P\<^isub>e\<^isub>r\<^isub>s\<^isub>o\<^isub>n4(*, X\<^isub>P\<^isub>e\<^isub>r\<^isub>s\<^isub>o\<^isub>n5*), X\<^isub>P\<^isub>e\<^isub>r\<^isub>s\<^isub>o\<^isub>n6, X\<^isub>P\<^isub>e\<^isub>r\<^isub>s\<^isub>o\<^isub>n7 .oclAsType(Person) })"
 proof -
  have p0 : "\<And>S oid\<^isub>8 oid\<^isub>7 person8 person7. oid\<^isub>8 \<noteq> oid\<^isub>7 \<Longrightarrow>
             S (oid\<^isub>8 \<mapsto> person8) (oid\<^isub>7 \<mapsto> person7) = S (oid\<^isub>7 \<mapsto> person7) (oid\<^isub>8 \<mapsto> person8)"
@@ -1011,93 +1010,25 @@ proof -
 
  fix \<sigma>\<^isub>1
  have eq : "Person .allInstances() (\<sigma>\<^isub>1,\<sigma>\<^isub>1') =
-       Set{X\<^isub>P\<^isub>e\<^isub>r\<^isub>s\<^isub>o\<^isub>n1, X\<^isub>P\<^isub>e\<^isub>r\<^isub>s\<^isub>o\<^isub>n2, X\<^isub>P\<^isub>e\<^isub>r\<^isub>s\<^isub>o\<^isub>n3, X\<^isub>P\<^isub>e\<^isub>r\<^isub>s\<^isub>o\<^isub>n4(*, X\<^isub>P\<^isub>e\<^isub>r\<^isub>s\<^isub>o\<^isub>n5*), X\<^isub>P\<^isub>e\<^isub>r\<^isub>s\<^isub>o\<^isub>n6, X\<^isub>P\<^isub>e\<^isub>r\<^isub>s\<^isub>o\<^isub>n7 .oclAsType(Person), \<lambda>_. \<lfloor>\<lfloor>Person (in\<^isub>o\<^isub>c\<^isub>l\<^isub>a\<^isub>n\<^isub>y person8)\<rfloor>\<rfloor>} (\<sigma>\<^isub>1,\<sigma>\<^isub>1')"
-  apply(simp only: perm)
-  apply(simp add: oid\<^isub>1_def oid\<^isub>2_def oid\<^isub>3_def oid\<^isub>4_def oid\<^isub>5_def oid\<^isub>6_def oid\<^isub>7_def oid\<^isub>8_def
-                  X\<^isub>P\<^isub>e\<^isub>r\<^isub>s\<^isub>o\<^isub>n1_def X\<^isub>P\<^isub>e\<^isub>r\<^isub>s\<^isub>o\<^isub>n2_def X\<^isub>P\<^isub>e\<^isub>r\<^isub>s\<^isub>o\<^isub>n3_def X\<^isub>P\<^isub>e\<^isub>r\<^isub>s\<^isub>o\<^isub>n4_def X\<^isub>P\<^isub>e\<^isub>r\<^isub>s\<^isub>o\<^isub>n5_def X\<^isub>P\<^isub>e\<^isub>r\<^isub>s\<^isub>o\<^isub>n6_def X\<^isub>P\<^isub>e\<^isub>r\<^isub>s\<^isub>o\<^isub>n7_def X\<^isub>P\<^isub>e\<^isub>r\<^isub>s\<^isub>o\<^isub>n8_def)
-  apply(subst state_update_vs_allInstances_rec, simp)+
-  apply(simp add: state_update_vs_allInstances_rec0)
-
-  apply(subst including_cp_all
-                                         ) prefer 4 apply(subst cp_OclIncluding[symmetric])
-  apply(subst including_cp_all[of _ _ _ "(\<sigma>\<^isub>1, \<lparr>heap = [7 \<mapsto> in\<^isub>o\<^isub>c\<^isub>l\<^isub>a\<^isub>n\<^isub>y person8],
-                    assocs = Map.empty\<rparr>)"]) prefer 4 apply(subst cp_OclIncluding[symmetric])
-  apply(subst including_cp_all[of _ _ _ "(\<sigma>\<^isub>1, \<lparr>heap = [7 \<mapsto> in\<^isub>o\<^isub>c\<^isub>l\<^isub>a\<^isub>n\<^isub>y person8, 6 \<mapsto> in\<^isub>o\<^isub>c\<^isub>l\<^isub>a\<^isub>n\<^isub>y person7],
-                    assocs = Map.empty\<rparr>)"]) prefer 4 apply(subst cp_OclIncluding[symmetric])
-  apply(subst including_cp_all[of _ _ _ "(\<sigma>\<^isub>1, \<lparr>heap = [7 \<mapsto> in\<^isub>o\<^isub>c\<^isub>l\<^isub>a\<^isub>n\<^isub>y person8, 6 \<mapsto> in\<^isub>o\<^isub>c\<^isub>l\<^isub>a\<^isub>n\<^isub>y person7, 5 \<mapsto> in\<^isub>p\<^isub>e\<^isub>r\<^isub>s\<^isub>o\<^isub>n person6],
-                    assocs = Map.empty\<rparr>)"]) prefer 4 apply(subst cp_OclIncluding[symmetric])
-  apply(subst including_cp_all[of _ _ _ "(\<sigma>\<^isub>1, \<lparr>heap = [7 \<mapsto> in\<^isub>o\<^isub>c\<^isub>l\<^isub>a\<^isub>n\<^isub>y person8, 6 \<mapsto> in\<^isub>o\<^isub>c\<^isub>l\<^isub>a\<^isub>n\<^isub>y person7, 5 \<mapsto> in\<^isub>p\<^isub>e\<^isub>r\<^isub>s\<^isub>o\<^isub>n person6, 3 \<mapsto> in\<^isub>p\<^isub>e\<^isub>r\<^isub>s\<^isub>o\<^isub>n person4],
-                    assocs = Map.empty\<rparr>)"]) prefer 4 apply(subst cp_OclIncluding[symmetric])
-  apply(subst including_cp_all[of _ _ _ "(\<sigma>\<^isub>1, \<lparr>heap = [7 \<mapsto> in\<^isub>o\<^isub>c\<^isub>l\<^isub>a\<^isub>n\<^isub>y person8, 6 \<mapsto> in\<^isub>o\<^isub>c\<^isub>l\<^isub>a\<^isub>n\<^isub>y person7, 5 \<mapsto> in\<^isub>p\<^isub>e\<^isub>r\<^isub>s\<^isub>o\<^isub>n person6, 3 \<mapsto> in\<^isub>p\<^isub>e\<^isub>r\<^isub>s\<^isub>o\<^isub>n person4, 2 \<mapsto> in\<^isub>p\<^isub>e\<^isub>r\<^isub>s\<^isub>o\<^isub>n person3],
-                    assocs = Map.empty\<rparr>)"]) prefer 4 apply(subst cp_OclIncluding[symmetric])
-  apply(subst including_cp_all[of _ _ _ "(\<sigma>\<^isub>1, \<lparr>heap = [7 \<mapsto> in\<^isub>o\<^isub>c\<^isub>l\<^isub>a\<^isub>n\<^isub>y person8, 6 \<mapsto> in\<^isub>o\<^isub>c\<^isub>l\<^isub>a\<^isub>n\<^isub>y person7, 5 \<mapsto> in\<^isub>p\<^isub>e\<^isub>r\<^isub>s\<^isub>o\<^isub>n person6, 3 \<mapsto> in\<^isub>p\<^isub>e\<^isub>r\<^isub>s\<^isub>o\<^isub>n person4, 2 \<mapsto> in\<^isub>p\<^isub>e\<^isub>r\<^isub>s\<^isub>o\<^isub>n person3, Suc 0 \<mapsto> in\<^isub>p\<^isub>e\<^isub>r\<^isub>s\<^isub>o\<^isub>n person2],
-                    assocs = Map.empty\<rparr>)"]) prefer 4 apply(subst cp_OclIncluding[symmetric])
-  apply(subst including_cp_all[of _ _ _ "(\<sigma>\<^isub>1, \<lparr>heap = [7 \<mapsto> in\<^isub>o\<^isub>c\<^isub>l\<^isub>a\<^isub>n\<^isub>y person8, 6 \<mapsto> in\<^isub>o\<^isub>c\<^isub>l\<^isub>a\<^isub>n\<^isub>y person7, 5 \<mapsto> in\<^isub>p\<^isub>e\<^isub>r\<^isub>s\<^isub>o\<^isub>n person6, 3 \<mapsto> in\<^isub>p\<^isub>e\<^isub>r\<^isub>s\<^isub>o\<^isub>n person4, 2 \<mapsto> in\<^isub>p\<^isub>e\<^isub>r\<^isub>s\<^isub>o\<^isub>n person3, Suc 0 \<mapsto> in\<^isub>p\<^isub>e\<^isub>r\<^isub>s\<^isub>o\<^isub>n person2, 0 \<mapsto> in\<^isub>p\<^isub>e\<^isub>r\<^isub>s\<^isub>o\<^isub>n person1],
-                    assocs = Map.empty\<rparr>)"]) prefer 4 apply(subst cp_OclIncluding[symmetric])
-
-  apply(simp add: person1_def person2_def person3_def person4_def person5_def person6_def person7_def person8_def)
-  apply(simp_all add: is_int_def)
-  apply((rule including_cp_all, simp_all add: is_int_def)+, simp add: mtSet_def)+
-  apply(simp add: mtSet_def) apply(simp add: mtSet_def)
- by (metis (no_types) foundation1 foundation16 mtSet_defined)
-
- show "?thesis \<sigma>\<^isub>1"
-  apply(simp only: StrictRefEq\<^isub>s\<^isub>e\<^isub>t StrongEq_def true_def OclValid_def)
-  apply(subst cp_valid)
-  apply(subst (1 2) eq)
-  apply(subst cp_valid[symmetric])
-  apply(simp add: X\<^isub>P\<^isub>e\<^isub>r\<^isub>s\<^isub>o\<^isub>n1_def X\<^isub>P\<^isub>e\<^isub>r\<^isub>s\<^isub>o\<^isub>n2_def X\<^isub>P\<^isub>e\<^isub>r\<^isub>s\<^isub>o\<^isub>n3_def X\<^isub>P\<^isub>e\<^isub>r\<^isub>s\<^isub>o\<^isub>n4_def X\<^isub>P\<^isub>e\<^isub>r\<^isub>s\<^isub>o\<^isub>n5_def X\<^isub>P\<^isub>e\<^isub>r\<^isub>s\<^isub>o\<^isub>n6_def X\<^isub>P\<^isub>e\<^isub>r\<^isub>s\<^isub>o\<^isub>n7_def X\<^isub>P\<^isub>e\<^isub>r\<^isub>s\<^isub>o\<^isub>n8_def
-                  person1_def person2_def person3_def person4_def person5_def person6_def person7_def person8_def)
- done
-qed
-
-lemma "\<And>\<sigma>\<^isub>1.    (\<sigma>\<^isub>1,\<sigma>\<^isub>1') \<Turnstile>      (OclAllInstances' Person' \<doteq> Set{ X\<^isub>P\<^isub>e\<^isub>r\<^isub>s\<^isub>o\<^isub>n1, X\<^isub>P\<^isub>e\<^isub>r\<^isub>s\<^isub>o\<^isub>n2, X\<^isub>P\<^isub>e\<^isub>r\<^isub>s\<^isub>o\<^isub>n3, X\<^isub>P\<^isub>e\<^isub>r\<^isub>s\<^isub>o\<^isub>n4(*, X\<^isub>P\<^isub>e\<^isub>r\<^isub>s\<^isub>o\<^isub>n5*), X\<^isub>P\<^isub>e\<^isub>r\<^isub>s\<^isub>o\<^isub>n6, X\<^isub>P\<^isub>e\<^isub>r\<^isub>s\<^isub>o\<^isub>n7 .oclAsType(Person) })"
-proof -
- have p0 : "\<And>S oid\<^isub>8 oid\<^isub>7 person8 person7. oid\<^isub>8 \<noteq> oid\<^isub>7 \<Longrightarrow>
-            S (oid\<^isub>8 \<mapsto> person8) (oid\<^isub>7 \<mapsto> person7) = S (oid\<^isub>7 \<mapsto> person7) (oid\<^isub>8 \<mapsto> person8)"
- by (metis fun_upd_twist)
-
- have perm : "\<sigma>\<^isub>1' = \<lparr> heap = empty
-                           (oid\<^isub>8 \<mapsto> in\<^isub>o\<^isub>c\<^isub>l\<^isub>a\<^isub>n\<^isub>y person8)
-                           (oid\<^isub>7 \<mapsto> in\<^isub>o\<^isub>c\<^isub>l\<^isub>a\<^isub>n\<^isub>y person7)
-                           (oid\<^isub>6 \<mapsto> in\<^isub>p\<^isub>e\<^isub>r\<^isub>s\<^isub>o\<^isub>n person6)
-                          (*oid\<^isub>5*)
-                           (oid\<^isub>4 \<mapsto> in\<^isub>p\<^isub>e\<^isub>r\<^isub>s\<^isub>o\<^isub>n person4)
-                           (oid\<^isub>3 \<mapsto> in\<^isub>p\<^isub>e\<^isub>r\<^isub>s\<^isub>o\<^isub>n person3)
-                           (oid\<^isub>2 \<mapsto> in\<^isub>p\<^isub>e\<^isub>r\<^isub>s\<^isub>o\<^isub>n person2)
-                           (oid\<^isub>1 \<mapsto> in\<^isub>p\<^isub>e\<^isub>r\<^isub>s\<^isub>o\<^isub>n person1)
-                , assocs = empty \<rparr>"
-  apply(simp add: \<sigma>\<^isub>1'_def
-                  oid\<^isub>1_def oid\<^isub>2_def oid\<^isub>3_def oid\<^isub>4_def oid\<^isub>5_def oid\<^isub>6_def oid\<^isub>7_def oid\<^isub>8_def)
-  apply(subst (1) p0, simp)
-  apply(subst (2) p0, simp) apply(subst (1) p0, simp)
-  apply(subst (3) p0, simp) apply(subst (2) p0, simp) apply(subst (1) p0, simp)
-  apply(subst (4) p0, simp) apply(subst (3) p0, simp) apply(subst (2) p0, simp) apply(subst (1) p0, simp)
-  apply(subst (5) p0, simp) apply(subst (4) p0, simp) apply(subst (3) p0, simp) apply(subst (2) p0, simp) apply(subst (1) p0, simp)
-  apply(subst (6) p0, simp) apply(subst (5) p0, simp) apply(subst (4) p0, simp) apply(subst (3) p0, simp) apply(subst (2) p0, simp) apply(subst (1) p0, simp)
- by(simp)
-
- fix \<sigma>\<^isub>1
- have eq : "OclAllInstances' Person' (\<sigma>\<^isub>1,\<sigma>\<^isub>1') =
        Set{X\<^isub>P\<^isub>e\<^isub>r\<^isub>s\<^isub>o\<^isub>n1, X\<^isub>P\<^isub>e\<^isub>r\<^isub>s\<^isub>o\<^isub>n2, X\<^isub>P\<^isub>e\<^isub>r\<^isub>s\<^isub>o\<^isub>n3, X\<^isub>P\<^isub>e\<^isub>r\<^isub>s\<^isub>o\<^isub>n4(*, X\<^isub>P\<^isub>e\<^isub>r\<^isub>s\<^isub>o\<^isub>n5*), X\<^isub>P\<^isub>e\<^isub>r\<^isub>s\<^isub>o\<^isub>n6, X\<^isub>P\<^isub>e\<^isub>r\<^isub>s\<^isub>o\<^isub>n7 .oclAsType(Person)} (\<sigma>\<^isub>1,\<sigma>\<^isub>1')"
   apply(simp only: perm)
   apply(simp add: oid\<^isub>1_def oid\<^isub>2_def oid\<^isub>3_def oid\<^isub>4_def oid\<^isub>5_def oid\<^isub>6_def oid\<^isub>7_def oid\<^isub>8_def
                   X\<^isub>P\<^isub>e\<^isub>r\<^isub>s\<^isub>o\<^isub>n1_def X\<^isub>P\<^isub>e\<^isub>r\<^isub>s\<^isub>o\<^isub>n2_def X\<^isub>P\<^isub>e\<^isub>r\<^isub>s\<^isub>o\<^isub>n3_def X\<^isub>P\<^isub>e\<^isub>r\<^isub>s\<^isub>o\<^isub>n4_def X\<^isub>P\<^isub>e\<^isub>r\<^isub>s\<^isub>o\<^isub>n5_def X\<^isub>P\<^isub>e\<^isub>r\<^isub>s\<^isub>o\<^isub>n6_def X\<^isub>P\<^isub>e\<^isub>r\<^isub>s\<^isub>o\<^isub>n7_def X\<^isub>P\<^isub>e\<^isub>r\<^isub>s\<^isub>o\<^isub>n8_def)
-  apply(subst state_update_vs_allInstances'_rec, simp, simp add: Person'_def
+  apply(subst state_update_vs_allInstances_including, simp, simp add: Person_def
    person1_def person2_def person3_def person4_def person5_def person6_def person7_def person8_def)
-  apply(subst state_update_vs_allInstances'_rec, simp, simp add: Person'_def
+  apply(subst state_update_vs_allInstances_including, simp, simp add: Person_def
    person1_def person2_def person3_def person4_def person5_def person6_def person7_def person8_def)
-  apply(subst state_update_vs_allInstances'_rec, simp, simp add: Person'_def
+  apply(subst state_update_vs_allInstances_including, simp, simp add: Person_def
    person1_def person2_def person3_def person4_def person5_def person6_def person7_def person8_def)
-  apply(subst state_update_vs_allInstances'_rec, simp, simp add: Person'_def
+  apply(subst state_update_vs_allInstances_including, simp, simp add: Person_def
    person1_def person2_def person3_def person4_def person5_def person6_def person7_def person8_def)
-  apply(subst state_update_vs_allInstances'_rec, simp, simp add: Person'_def
+  apply(subst state_update_vs_allInstances_including, simp, simp add: Person_def
    person1_def person2_def person3_def person4_def person5_def person6_def person7_def person8_def)
-  apply(subst state_update_vs_allInstances'_rec, simp, simp add: Person'_def
+  apply(subst state_update_vs_allInstances_including, simp, simp add: Person_def
    person1_def person2_def person3_def person4_def person5_def person6_def person7_def person8_def)
-  apply(subst state_update_vs_allInstances'_recnone, simp, simp add: Person'_def
+  apply(subst state_update_vs_allInstances_noincluding, simp, simp add: Person_def
    person1_def person2_def person3_def person4_def person5_def person6_def person7_def person8_def)
-  apply(subst state_update_vs_allInstances'_rec0)
+  apply(subst state_update_vs_allInstances_empty)
 
   apply(subst including_cp_all
                                          ) prefer 4 apply(subst cp_OclIncluding[symmetric])
@@ -1116,7 +1047,7 @@ proof -
   apply(subst including_cp_all[of _ _ _ "(\<sigma>\<^isub>1, \<lparr>heap = [7 \<mapsto> in\<^isub>o\<^isub>c\<^isub>l\<^isub>a\<^isub>n\<^isub>y person8, 6 \<mapsto> in\<^isub>o\<^isub>c\<^isub>l\<^isub>a\<^isub>n\<^isub>y person7, 5 \<mapsto> in\<^isub>p\<^isub>e\<^isub>r\<^isub>s\<^isub>o\<^isub>n person6, 3 \<mapsto> in\<^isub>p\<^isub>e\<^isub>r\<^isub>s\<^isub>o\<^isub>n person4, 2 \<mapsto> in\<^isub>p\<^isub>e\<^isub>r\<^isub>s\<^isub>o\<^isub>n person3, Suc 0 \<mapsto> in\<^isub>p\<^isub>e\<^isub>r\<^isub>s\<^isub>o\<^isub>n person2, 0 \<mapsto> in\<^isub>p\<^isub>e\<^isub>r\<^isub>s\<^isub>o\<^isub>n person1],
                     assocs = Map.empty\<rparr>)"]) prefer 4 apply(subst cp_OclIncluding[symmetric])
 
-  apply(simp add: Person'_def person1_def person2_def person3_def person4_def person5_def person6_def person7_def person8_def)
+  apply(simp add: Person_def person1_def person2_def person3_def person4_def person5_def person6_def person7_def person8_def)
   apply(simp_all add: is_int_def)
   apply((rule including_cp_all, simp_all add: is_int_def)+, simp add: mtSet_def)+
   apply(simp add: mtSet_def) apply(simp add: mtSet_def) apply(simp add: mtSet_def)
@@ -1132,7 +1063,7 @@ proof -
  done
 qed
 
-lemma "\<And>\<sigma>\<^isub>1.    (\<sigma>\<^isub>1,\<sigma>\<^isub>1') \<Turnstile>      (OclAllInstances' OclAny' \<doteq> Set{ X\<^isub>P\<^isub>e\<^isub>r\<^isub>s\<^isub>o\<^isub>n1 .oclAsType(OclAny), X\<^isub>P\<^isub>e\<^isub>r\<^isub>s\<^isub>o\<^isub>n2 .oclAsType(OclAny), X\<^isub>P\<^isub>e\<^isub>r\<^isub>s\<^isub>o\<^isub>n3 .oclAsType(OclAny), X\<^isub>P\<^isub>e\<^isub>r\<^isub>s\<^isub>o\<^isub>n4 .oclAsType(OclAny)(*, X\<^isub>P\<^isub>e\<^isub>r\<^isub>s\<^isub>o\<^isub>n5*), X\<^isub>P\<^isub>e\<^isub>r\<^isub>s\<^isub>o\<^isub>n6 .oclAsType(OclAny), X\<^isub>P\<^isub>e\<^isub>r\<^isub>s\<^isub>o\<^isub>n7, X\<^isub>P\<^isub>e\<^isub>r\<^isub>s\<^isub>o\<^isub>n8 })"
+lemma "\<And>\<sigma>\<^isub>1.    (\<sigma>\<^isub>1,\<sigma>\<^isub>1') \<Turnstile>      (OclAny .allInstances() \<doteq> Set{ X\<^isub>P\<^isub>e\<^isub>r\<^isub>s\<^isub>o\<^isub>n1 .oclAsType(OclAny), X\<^isub>P\<^isub>e\<^isub>r\<^isub>s\<^isub>o\<^isub>n2 .oclAsType(OclAny), X\<^isub>P\<^isub>e\<^isub>r\<^isub>s\<^isub>o\<^isub>n3 .oclAsType(OclAny), X\<^isub>P\<^isub>e\<^isub>r\<^isub>s\<^isub>o\<^isub>n4 .oclAsType(OclAny)(*, X\<^isub>P\<^isub>e\<^isub>r\<^isub>s\<^isub>o\<^isub>n5*), X\<^isub>P\<^isub>e\<^isub>r\<^isub>s\<^isub>o\<^isub>n6 .oclAsType(OclAny), X\<^isub>P\<^isub>e\<^isub>r\<^isub>s\<^isub>o\<^isub>n7, X\<^isub>P\<^isub>e\<^isub>r\<^isub>s\<^isub>o\<^isub>n8 })"
 proof -
  have p0 : "\<And>S oid\<^isub>8 oid\<^isub>7 person8 person7. oid\<^isub>8 \<noteq> oid\<^isub>7 \<Longrightarrow>
             S (oid\<^isub>8 \<mapsto> person8) (oid\<^isub>7 \<mapsto> person7) = S (oid\<^isub>7 \<mapsto> person7) (oid\<^isub>8 \<mapsto> person8)"
@@ -1159,26 +1090,26 @@ proof -
  by(simp)
 
  fix \<sigma>\<^isub>1
- have eq : "OclAllInstances' OclAny' (\<sigma>\<^isub>1,\<sigma>\<^isub>1') =
+ have eq : "OclAny .allInstances() (\<sigma>\<^isub>1,\<sigma>\<^isub>1') =
        Set{ X\<^isub>P\<^isub>e\<^isub>r\<^isub>s\<^isub>o\<^isub>n1 .oclAsType(OclAny), X\<^isub>P\<^isub>e\<^isub>r\<^isub>s\<^isub>o\<^isub>n2 .oclAsType(OclAny), X\<^isub>P\<^isub>e\<^isub>r\<^isub>s\<^isub>o\<^isub>n3 .oclAsType(OclAny), X\<^isub>P\<^isub>e\<^isub>r\<^isub>s\<^isub>o\<^isub>n4 .oclAsType(OclAny)(*, X\<^isub>P\<^isub>e\<^isub>r\<^isub>s\<^isub>o\<^isub>n5*), X\<^isub>P\<^isub>e\<^isub>r\<^isub>s\<^isub>o\<^isub>n6 .oclAsType(OclAny), X\<^isub>P\<^isub>e\<^isub>r\<^isub>s\<^isub>o\<^isub>n7, X\<^isub>P\<^isub>e\<^isub>r\<^isub>s\<^isub>o\<^isub>n8 } (\<sigma>\<^isub>1,\<sigma>\<^isub>1')"
   apply(simp only: perm)
   apply(simp add: oid\<^isub>1_def oid\<^isub>2_def oid\<^isub>3_def oid\<^isub>4_def oid\<^isub>5_def oid\<^isub>6_def oid\<^isub>7_def oid\<^isub>8_def
                   X\<^isub>P\<^isub>e\<^isub>r\<^isub>s\<^isub>o\<^isub>n1_def X\<^isub>P\<^isub>e\<^isub>r\<^isub>s\<^isub>o\<^isub>n2_def X\<^isub>P\<^isub>e\<^isub>r\<^isub>s\<^isub>o\<^isub>n3_def X\<^isub>P\<^isub>e\<^isub>r\<^isub>s\<^isub>o\<^isub>n4_def X\<^isub>P\<^isub>e\<^isub>r\<^isub>s\<^isub>o\<^isub>n5_def X\<^isub>P\<^isub>e\<^isub>r\<^isub>s\<^isub>o\<^isub>n6_def X\<^isub>P\<^isub>e\<^isub>r\<^isub>s\<^isub>o\<^isub>n7_def X\<^isub>P\<^isub>e\<^isub>r\<^isub>s\<^isub>o\<^isub>n8_def)
-  apply(subst state_update_vs_allInstances'_rec, simp, simp add: OclAny'_def
+  apply(subst state_update_vs_allInstances_including, simp, simp add: OclAny_def
    person1_def person2_def person3_def person4_def person5_def person6_def person7_def person8_def)
-  apply(subst state_update_vs_allInstances'_rec, simp, simp add: OclAny'_def
+  apply(subst state_update_vs_allInstances_including, simp, simp add: OclAny_def
    person1_def person2_def person3_def person4_def person5_def person6_def person7_def person8_def)
-  apply(subst state_update_vs_allInstances'_rec, simp, simp add: OclAny'_def
+  apply(subst state_update_vs_allInstances_including, simp, simp add: OclAny_def
    person1_def person2_def person3_def person4_def person5_def person6_def person7_def person8_def)
-  apply(subst state_update_vs_allInstances'_rec, simp, simp add: OclAny'_def
+  apply(subst state_update_vs_allInstances_including, simp, simp add: OclAny_def
    person1_def person2_def person3_def person4_def person5_def person6_def person7_def person8_def)
-  apply(subst state_update_vs_allInstances'_rec, simp, simp add: OclAny'_def
+  apply(subst state_update_vs_allInstances_including, simp, simp add: OclAny_def
    person1_def person2_def person3_def person4_def person5_def person6_def person7_def person8_def)
-  apply(subst state_update_vs_allInstances'_rec, simp, simp add: OclAny'_def
+  apply(subst state_update_vs_allInstances_including, simp, simp add: OclAny_def
    person1_def person2_def person3_def person4_def person5_def person6_def person7_def person8_def)
-  apply(subst state_update_vs_allInstances'_rec, simp, simp add: OclAny'_def
+  apply(subst state_update_vs_allInstances_including, simp, simp add: OclAny_def
    person1_def person2_def person3_def person4_def person5_def person6_def person7_def person8_def)
-  apply(subst state_update_vs_allInstances'_rec0)
+  apply(subst state_update_vs_allInstances_empty)
 
   apply(subst including_cp_all
                                          ) prefer 4 apply(subst cp_OclIncluding[symmetric])
@@ -1197,7 +1128,7 @@ proof -
   apply(subst including_cp_all[of _ _ _ "(\<sigma>\<^isub>1, \<lparr>heap = [7 \<mapsto> in\<^isub>o\<^isub>c\<^isub>l\<^isub>a\<^isub>n\<^isub>y person8, 6 \<mapsto> in\<^isub>o\<^isub>c\<^isub>l\<^isub>a\<^isub>n\<^isub>y person7, 5 \<mapsto> in\<^isub>p\<^isub>e\<^isub>r\<^isub>s\<^isub>o\<^isub>n person6, 3 \<mapsto> in\<^isub>p\<^isub>e\<^isub>r\<^isub>s\<^isub>o\<^isub>n person4, 2 \<mapsto> in\<^isub>p\<^isub>e\<^isub>r\<^isub>s\<^isub>o\<^isub>n person3, Suc 0 \<mapsto> in\<^isub>p\<^isub>e\<^isub>r\<^isub>s\<^isub>o\<^isub>n person2, 0 \<mapsto> in\<^isub>p\<^isub>e\<^isub>r\<^isub>s\<^isub>o\<^isub>n person1],
                     assocs = Map.empty\<rparr>)"]) prefer 4 apply(subst cp_OclIncluding[symmetric])
 
-  apply(simp add: OclAny'_def person1_def person2_def person3_def person4_def person5_def person6_def person7_def person8_def)
+  apply(simp add: OclAny_def person1_def person2_def person3_def person4_def person5_def person6_def person7_def person8_def)
   apply(simp_all add: is_int_def)
   apply((rule including_cp_all, simp_all add: is_int_def)+, simp add: mtSet_def)+
   apply(simp add: mtSet_def) apply(simp add: mtSet_def)
@@ -1211,59 +1142,6 @@ proof -
   apply(simp add: X\<^isub>P\<^isub>e\<^isub>r\<^isub>s\<^isub>o\<^isub>n1_def X\<^isub>P\<^isub>e\<^isub>r\<^isub>s\<^isub>o\<^isub>n2_def X\<^isub>P\<^isub>e\<^isub>r\<^isub>s\<^isub>o\<^isub>n3_def X\<^isub>P\<^isub>e\<^isub>r\<^isub>s\<^isub>o\<^isub>n4_def X\<^isub>P\<^isub>e\<^isub>r\<^isub>s\<^isub>o\<^isub>n5_def X\<^isub>P\<^isub>e\<^isub>r\<^isub>s\<^isub>o\<^isub>n6_def X\<^isub>P\<^isub>e\<^isub>r\<^isub>s\<^isub>o\<^isub>n7_def X\<^isub>P\<^isub>e\<^isub>r\<^isub>s\<^isub>o\<^isub>n8_def
                   person1_def person2_def person3_def person4_def person5_def person6_def person7_def person8_def)
  done
-qed
-
-
-
-
-lemma
- fixes \<sigma>\<^isub>1 \<sigma>\<^isub>1'
-       person0 person1 person2
-       X\<^isub>P\<^isub>e\<^isub>r\<^isub>s\<^isub>o\<^isub>n0 X\<^isub>P\<^isub>e\<^isub>r\<^isub>s\<^isub>o\<^isub>n1 X\<^isub>P\<^isub>e\<^isub>r\<^isub>s\<^isub>o\<^isub>n2
- defines "person0 \<equiv> mk\<^isub>o\<^isub>c\<^isub>l\<^isub>a\<^isub>n\<^isub>y 0 None"
- defines "person1 \<equiv> mk\<^isub>o\<^isub>c\<^isub>l\<^isub>a\<^isub>n\<^isub>y 1 \<lfloor>(\<lfloor>20\<rfloor>, \<lfloor>2\<rfloor>)\<rfloor>"
- defines "person2 \<equiv> mk\<^isub>p\<^isub>e\<^isub>r\<^isub>s\<^isub>o\<^isub>n 2 \<lfloor>30\<rfloor> \<lfloor>1\<rfloor>"
- defines "\<sigma>\<^isub>1' \<equiv> \<lparr> heap = empty(0 \<mapsto> in\<^isub>o\<^isub>c\<^isub>l\<^isub>a\<^isub>n\<^isub>y person0)
-                              (1 \<mapsto> in\<^isub>o\<^isub>c\<^isub>l\<^isub>a\<^isub>n\<^isub>y person1)
-                              (2 \<mapsto> in\<^isub>p\<^isub>e\<^isub>r\<^isub>s\<^isub>o\<^isub>n person2)
-                , assocs = empty \<rparr>"
- defines "X\<^isub>P\<^isub>e\<^isub>r\<^isub>s\<^isub>o\<^isub>n0 \<equiv> (\<lambda>_. \<lfloor>\<lfloor> person0 \<rfloor>\<rfloor>)"
- defines "X\<^isub>P\<^isub>e\<^isub>r\<^isub>s\<^isub>o\<^isub>n1 \<equiv> (\<lambda>_. \<lfloor>\<lfloor> person1 \<rfloor>\<rfloor>)"
- defines "X\<^isub>P\<^isub>e\<^isub>r\<^isub>s\<^isub>o\<^isub>n2 :: Person \<equiv> (\<lambda>_. \<lfloor>\<lfloor> person2 \<rfloor>\<rfloor>)"
- shows "(OclAny .allInstances()) (\<sigma>\<^isub>1,\<sigma>\<^isub>1') = Set{X\<^isub>P\<^isub>e\<^isub>r\<^isub>s\<^isub>o\<^isub>n0, X\<^isub>P\<^isub>e\<^isub>r\<^isub>s\<^isub>o\<^isub>n1, X\<^isub>P\<^isub>e\<^isub>r\<^isub>s\<^isub>o\<^isub>n2 .oclAsType(OclAny)} (\<sigma>\<^isub>1,\<sigma>\<^isub>1')"
-proof -
- have perm : "\<sigma>\<^isub>1' = \<lparr> heap = empty(2 \<mapsto> in\<^isub>p\<^isub>e\<^isub>r\<^isub>s\<^isub>o\<^isub>n person2)
-                                 (1 \<mapsto> in\<^isub>o\<^isub>c\<^isub>l\<^isub>a\<^isub>n\<^isub>y person1)
-                                 (0 \<mapsto> in\<^isub>o\<^isub>c\<^isub>l\<^isub>a\<^isub>n\<^isub>y person0)
-                , assocs = empty \<rparr>"
-  apply(simp add: \<sigma>\<^isub>1'_def)
-  proof -
-  have "Suc 0 = oid\<^isub>2" by (metis One_nat_def oid\<^isub>2_def)
-  thus "[0 \<mapsto> in\<^isub>o\<^isub>c\<^isub>l\<^isub>a\<^isub>n\<^isub>y person0, Suc 0 \<mapsto> in\<^isub>o\<^isub>c\<^isub>l\<^isub>a\<^isub>n\<^isub>y person1, 2 \<mapsto> in\<^isub>p\<^isub>e\<^isub>r\<^isub>s\<^isub>o\<^isub>n person2] = [2 \<mapsto> in\<^isub>p\<^isub>e\<^isub>r\<^isub>s\<^isub>o\<^isub>n person2, Suc 0 \<mapsto> in\<^isub>o\<^isub>c\<^isub>l\<^isub>a\<^isub>n\<^isub>y person1, 0 \<mapsto> in\<^isub>o\<^isub>c\<^isub>l\<^isub>a\<^isub>n\<^isub>y person0]"
-  by (metis One_nat_def Suc_1 Zero_not_Suc fun_upd_twist n_not_Suc_n zero_neq_numeral)
- qed
-
- show ?thesis
-  apply(simp only: perm)
-  apply(simp add: comp_def image_def \<sigma>\<^isub>1'_def X\<^isub>P\<^isub>e\<^isub>r\<^isub>s\<^isub>o\<^isub>n0_def X\<^isub>P\<^isub>e\<^isub>r\<^isub>s\<^isub>o\<^isub>n1_def X\<^isub>P\<^isub>e\<^isub>r\<^isub>s\<^isub>o\<^isub>n2_def)
-  apply(subst state_update_vs_allInstances_rec, simp)+
-  apply(simp add: state_update_vs_allInstances_rec0)
-
-  apply(subst including_cp_all
-                                         ) prefer 4 apply(subst cp_OclIncluding[symmetric])
-  apply(subst including_cp_all[of _ _ _ "(\<sigma>\<^isub>1, \<lparr>heap = [2 \<mapsto> in\<^isub>p\<^isub>e\<^isub>r\<^isub>s\<^isub>o\<^isub>n person2],
-                    assocs = Map.empty\<rparr>)"]) prefer 4 apply(subst cp_OclIncluding[symmetric])
-  apply(subst including_cp_all[of _ _ _ "(\<sigma>\<^isub>1, \<lparr>heap = [2 \<mapsto> in\<^isub>p\<^isub>e\<^isub>r\<^isub>s\<^isub>o\<^isub>n person2, Suc 0 \<mapsto> in\<^isub>o\<^isub>c\<^isub>l\<^isub>a\<^isub>n\<^isub>y person1],
-                    assocs = Map.empty\<rparr>)"]) prefer 4 apply(subst cp_OclIncluding[symmetric])
-  apply(subst including_cp_all[of _ _ _ "(\<sigma>\<^isub>1, \<lparr>heap = [2 \<mapsto> in\<^isub>p\<^isub>e\<^isub>r\<^isub>s\<^isub>o\<^isub>n person2, Suc 0 \<mapsto> in\<^isub>o\<^isub>c\<^isub>l\<^isub>a\<^isub>n\<^isub>y person1, 0 \<mapsto> in\<^isub>o\<^isub>c\<^isub>l\<^isub>a\<^isub>n\<^isub>y person0],
-                    assocs = Map.empty\<rparr>)"]) prefer 4 apply(subst cp_OclIncluding[symmetric])
-
-  apply(simp add: person2_def)
-  apply(simp_all add: is_int_def)
-  apply(rule including_cp_all)
-  apply(simp_all add: is_int_def)
-  apply(simp add: mtSet_def) apply(simp add: mtSet_def) apply(simp add: mtSet_def)
- by (metis (no_types) foundation1 foundation16 mtSet_defined)
 qed
 
 end
